work from last night.

MirrorCharge!/src/MirrorCharge/Imp/Bench_Mem.v
@@ -3,6 +3,7 @@ Require Import MirrorCharge.Imp.Goal.
 Require Import MirrorCharge.Imp.ImpTac.
 Require Import MirrorCharge.Imp.SymEvalLemmas.
 Require MirrorCharge.Imp.STacCancel.
+Require Import MirrorCharge.Imp.Syntax.
 
 Definition entailment_tac : imp_tac := THEN SIMPLIFY (runOnGoals STacCancel.stac_cancel).
 Definition simplify_tac : imp_tac := SIMPLIFY.
@@ -27,9 +28,9 @@ Definition EAPPLY_THEN_1 a (side : imp_tac) (b : imp_tacK) : imp_tac :=
                                                 end))))).
 
 Definition sym_eval_mem (n : nat) : imp_tac :=
-  REC n (fun rec : imp_tac =>
+  REC_N n (fun rec : imp_tac =>
            let rec := THEN simplify_tac (runOnGoals rec) in
-           FIRST (   EAPPLY SeqA_lemma
+           FIRST (   EAPPLY_THEN SeqA_lemma rec
                   :: EAPPLY_THEN Assign_seq_lemma rec
                   :: EAPPLY_THEN_1 Read_seq_lemma entailment_tac (runOnGoals rec)
                   :: EAPPLY_THEN_1 Write_seq_lemma entailment_tac (runOnGoals rec)
@@ -43,6 +44,8 @@ Definition sym_eval_mem (n : nat) : imp_tac :=
                   :: nil))
       IDTAC.
 
+
+
 Definition Prove P c Q :=
   App
     (App
@@ -50,8 +53,54 @@ Definition Prove P c Q :=
        (Reify._Inj (inr (ILogicFunc.ilf_true Syntax.tySProp))))
     (App (App (App Syntax.fTriple P) c) Q).
 
+Fixpoint skips (n : nat) :=
+  match n with
+    | 0 => Syntax.fSkip
+    | S n => App (App Syntax.fSeq Syntax.fSkip) (skips n)
+  end.
+
+Require Import Coq.Strings.String.
+
+Fixpoint adds_syn (n : nat) :=
+  match n with
+    | 0 => Syntax.fSkip
+    | S n => Syntax.mkSeq (Syntax.mkAssign (Syntax.fVar "x") (Syntax.fVar "x")) (adds_syn n)
+  end%string.
+
 Time Eval vm_compute in
     let tus := nil in
     let tvs := nil in
     let goal := Prove (Syntax.ltrue Syntax.tyLProp) Syntax.fSkip (Syntax.ltrue Syntax.tyLProp) in
     runImpTac tus tvs goal (sym_eval_mem 5).
+
+Time Eval vm_compute in
+    let tus := nil in
+    let tvs := nil in
+    let goal := Prove (Syntax.ltrue Syntax.tyLProp) (skips 800) (Syntax.ltrue Syntax.tyLProp) in
+    runImpTac tus tvs goal (sym_eval_mem 810).
+
+Time Eval vm_compute in
+    let n := 100 in
+    let tus := nil in
+    let tvs := nil in
+    let goal := Prove (Syntax.ltrue Syntax.tyLProp) (adds_syn n) (Syntax.ltrue Syntax.tyLProp) in
+    runImpTac tus tvs goal (sym_eval_mem n).
+
+Fixpoint adds (n : nat) :=
+  match n with
+    | 0 => Imp.Skip
+    | S n => Imp.Seq (Imp.Assign "x" (Imp.iVar "x")) (adds n)
+  end%string.
+
+Goal @ILogic.lentails Imp.SProp Imp.ILogicOps_SProp (@ILogic.ltrue Imp.SProp Imp.ILogicOps_SProp)
+     (Imp.triple (@ILogic.ltrue Imp.lprop Imp.ILogicOps_lprop)
+        (adds 10)
+        (@ILogic.ltrue Imp.lprop Imp.ILogicOps_lprop)).
+unfold adds.
+match goal with
+  | |- ?goal =>
+    let k g :=
+        pose g
+    in
+    reify_expr Reify.reify_imp k [ True ] [ goal ]
+end.
